wip on precise-gDot where wf-ness is not carried with wf_ctx, but only through regularity of typing --> no problems in narrow_wf with bigger env. Problem: We need a narrow_has cannot get wf-ness to return subtyp_refl etc, need to introduce a regularity mode for subtyp/subdec.

dev/existential/precise-gDot.v
@@ -26,11 +26,13 @@ Inductive avar : Set :=
 Inductive typ : Set :=
   | typ_top  : typ
   | typ_bot  : typ
-  | typ_tdec : typ_label -> typ -> typ -> typ (* { L: S..U } *)
-  | typ_mdec : mtd_label -> typ -> typ -> typ (* { m: S->U } *)
+  | typ_rcd  : dec -> typ (* { D } *)
   | typ_sel  : avar -> typ_label -> typ (* x.L *)
   | typ_and  : typ -> typ -> typ
-  | typ_or   : typ -> typ -> typ.
+  | typ_or   : typ -> typ -> typ
+with dec : Set :=
+  | dec_typ  : typ_label -> typ -> typ -> dec (* L: S..U *)
+  | dec_mtd  : mtd_label -> typ -> typ -> dec (* m: S->U *).
 
 Inductive trm: Set :=
   | trm_var : avar -> trm
@@ -60,6 +62,11 @@ Definition label_of_def(d: def): label := match d with
 | def_mtd m _ _ _ => label_mtd m
 end.
 
+Definition label_of_dec(D: dec): label := match D with
+| dec_typ L _ _ => label_typ L
+| dec_mtd m _ _ => label_mtd m
+end.
+
 Fixpoint get_def(l: label)(ds: defs): option def :=
 match ds with
 | defs_nil => None
@@ -86,11 +93,15 @@ Fixpoint open_rec_typ (k: nat) (u: var) (T: typ): typ :=
   match T with
   | typ_top        => typ_top
   | typ_bot        => typ_bot
-  | typ_tdec L T U => typ_tdec L (open_rec_typ k u T) (open_rec_typ k u U)
-  | typ_mdec m T U => typ_mdec m (open_rec_typ k u T) (open_rec_typ k u U)
+  | typ_rcd D      => typ_rcd (open_rec_dec k u D)
   | typ_sel x L    => typ_sel (open_rec_avar k u x) L
   | typ_and T1 T2  => typ_and (open_rec_typ k u T1) (open_rec_typ k u T2)
   | typ_or  T1 T2  => typ_or  (open_rec_typ k u T1) (open_rec_typ k u T2)
+  end
+with open_rec_dec (k: nat) (u: var) (D: dec): dec :=
+  match D with
+  | dec_typ L T U => dec_typ L (open_rec_typ k u T) (open_rec_typ k u U)
+  | dec_mtd m T U => dec_mtd m (open_rec_typ k u T) (open_rec_typ k u U)
   end.
 
 Fixpoint open_rec_trm (k: nat) (u: var) (t: trm): trm :=
@@ -114,6 +125,7 @@ with open_rec_defs (k: nat) (u: var) (ds: defs): defs :=
 
 Definition open_avar u a := open_rec_avar  0 u a.
 Definition open_typ  u t := open_rec_typ   0 u t.
+Definition open_dec  u D := open_rec_dec   0 u D.
 Definition open_trm  u e := open_rec_trm   0 u e.
 Definition open_def  u d := open_rec_def   0 u d.
 Definition open_defs u l := open_rec_defs  0 u l.
@@ -132,11 +144,15 @@ Fixpoint fv_typ (T: typ) : vars :=
   match T with
   | typ_top        => \{}
   | typ_bot        => \{}
-  | typ_tdec L T U => (fv_typ T) \u (fv_typ U)
-  | typ_mdec m T U => (fv_typ T) \u (fv_typ U)
+  | typ_rcd D      => (fv_dec D)
   | typ_sel x L    => (fv_avar x)
   | typ_and T U    => (fv_typ T) \u (fv_typ U)
   | typ_or  T U    => (fv_typ T) \u (fv_typ U)
+  end
+with fv_dec (D: dec) : vars :=
+  match D with
+  | dec_typ L T U => (fv_typ T) \u (fv_typ U)
+  | dec_mtd m T U => (fv_typ T) \u (fv_typ U)
   end.
 
 (* Since we define defs ourselves instead of using [list def], we don't have any
@@ -192,31 +208,213 @@ Inductive red : trm -> sto -> trm -> sto -> Prop :=
 (* ###################################################################### *)
 (** ** Typing *)
 
+(* "optimization" of typ_and (makes some proofs simpler, but others more
+    complicated!!).
+   If intersect_dec and thus typ_has uses intersect_typ instead of typ_and, 
+   we know that if a decl returned by typ_has is "equivalent" to a bottom-decl,
+   it's actually also structurally equal.
+   Or in other words: Instead of returning (dec_fld l (typ_and typ_bot T)),
+   typ_has will return just (dec_fld l typ_bot). *)
+Definition intersect_typ(T1 T2: typ): typ := If T1 = T2 then T1 else
+match T1, T2 with
+| typ_top, _ => T2
+| _, typ_top => T1
+| typ_bot, _ => typ_bot
+| _, typ_bot => typ_bot
+| _, _       => typ_and T1 T2
+end.
+
+Definition union_typ(T1 T2: typ): typ := If T1 = T2 then T1 else
+match T1, T2 with
+| typ_top, _ => typ_top
+| _, typ_top => typ_top
+| typ_bot, _ => T2
+| _, typ_bot => T1
+| _, _       => typ_or T1 T2
+end.
+
+(*
+(* returns (option dec) because it's not total. *)
+Definition intersect_dec(D1 D2: dec): option dec :=
+  If label_of_dec D1 = label_of_dec D2 then
+    match D1, D2 with
+    | (dec_typ L S1 U1), (dec_typ _ S2 U2)
+      => Some (dec_typ L (typ_or S1 S2) (typ_and U1 U2))
+    | (dec_mtd m S1 U1), (dec_mtd _ S2 U2)
+      => Some (dec_mtd m (typ_or S1 S2) (typ_and U1 U2))
+    | _, _ => None
+    end
+  else
+    None.
+
+Definition union_dec(D1 D2: dec): option dec :=
+  If label_of_dec D1 = label_of_dec D2 then
+    match D1, D2 with
+    | (dec_typ L S1 U1), (dec_typ _ S2 U2)
+      => Some (dec_typ L (typ_and S1 S2) (typ_or U1 U2))
+    | (dec_mtd m S1 U1), (dec_mtd _ S2 U2)
+      => Some (dec_mtd m (typ_and S1 S2) (typ_or U1 U2))
+    | _, _ => None
+    end
+  else
+    None.
+*)
+
+Definition intersect_dec(D1 D2: dec): option dec :=
+  If label_of_dec D1 = label_of_dec D2 then
+    match D1, D2 with
+    | (dec_typ L S1 U1), (dec_typ _ S2 U2)
+      => Some (dec_typ L (union_typ S1 S2) (intersect_typ U1 U2))
+    | (dec_mtd m S1 U1), (dec_mtd _ S2 U2)
+      => Some (dec_mtd m (union_typ S1 S2) (intersect_typ U1 U2))
+    | _, _ => None
+    end
+  else
+    None.
+
+Definition union_dec(D1 D2: dec): option dec :=
+  If label_of_dec D1 = label_of_dec D2 then
+    match D1, D2 with
+    | (dec_typ L S1 U1), (dec_typ _ S2 U2)
+      => Some (dec_typ L (intersect_typ S1 S2) (union_typ U1 U2))
+    | (dec_mtd m S1 U1), (dec_mtd _ S2 U2)
+      => Some (dec_mtd m (intersect_typ S1 S2) (union_typ U1 U2))
+    | _, _ => None
+    end
+  else
+    None.
+
+Notation "D1 && D2 == D3" := (intersect_dec D1 D2 = Some D3) (at level 40).
+Notation "D1 || D2 == D3" := (union_dec D1 D2 = Some D3) (at level 40).
+
+Definition dec_bot(l: label): dec := match l with
+  | label_typ L => dec_typ L typ_top typ_bot
+  | label_mtd m => dec_mtd m typ_top typ_bot
+end.
+
+(*
+Definition dec_top(l: label): dec := match l with
+  | label_typ L => dec_typ L typ_bot typ_top
+  | label_mtd m => dec_mtd m typ_bot typ_top
+end.
+*)
+
+Inductive typ_has: ctx -> typ -> dec -> Prop :=
+(*| typ_top_has: typ_top has nothing *)
+  | typ_bot_has: forall G l,
+      typ_has G typ_bot (dec_bot l)
+  | typ_rcd_has: forall G D,
+      typ_has G (typ_rcd D) D
+  | typ_sel_has: forall G x T L Lo Hi D,
+      binds x T G ->
+      typ_has  G T (dec_typ L Lo Hi) ->
+      typ_has  G Hi D ->
+      typ_has G (typ_sel (avar_f x) L) D
+  | typ_and_has_1: forall G T1 T2 D,
+      typ_has G T1 D ->
+      typ_hasnt G T2 (label_of_dec D) ->
+      typ_has G (typ_and T1 T2) D
+  | typ_and_has_2: forall G T1 T2 D,
+      typ_hasnt G T1 (label_of_dec D) ->
+      typ_has G T2 D ->
+      typ_has G (typ_and T1 T2) D
+  | typ_and_has_12: forall G T1 T2 D1 D2 D3,
+      typ_has G T1 D1 ->
+      typ_has G T2 D2 ->
+      D1 && D2 == D3 ->
+      typ_has G (typ_and T1 T2) D3
+  | typ_or_has: forall G T1 T2 D1 D2 D3,
+      typ_has G T1 D1 ->
+      typ_has G T2 D2 ->
+      D1 || D2 == D3 ->
+      typ_has G (typ_or T1 T2) D3
+with typ_hasnt: ctx -> typ -> label -> Prop :=
+  | typ_top_hasnt: forall G l,
+      typ_hasnt G typ_top l
+(*| typ_bot_hasnt: There's no label that typ_bot hasn't. *)
+  | typ_rcd_hasnt: forall G D l,
+      l <> label_of_dec D ->
+      typ_hasnt G (typ_rcd D) l
+  | typ_sel_hasnt: forall G x T L Lo Hi l,
+      binds x T G ->
+      typ_has    G T (dec_typ L Lo Hi) ->
+      typ_hasnt  G Hi l ->
+      typ_hasnt G (typ_sel (avar_f x) L) l
+  | typ_and_hasnt: forall G T1 T2 l, 
+      typ_hasnt G T1 l ->
+      typ_hasnt G T2 l ->
+      typ_hasnt G (typ_and T1 T2) l
+  | typ_or_hasnt_1: forall G T1 T2 l,
+      typ_hasnt G T1 l ->
+      typ_hasnt G (typ_or T1 T2) l
+  | typ_or_hasnt_2: forall G T1 T2 l,
+      typ_hasnt G T2 l ->
+      typ_hasnt G (typ_or T1 T2) l.
+
+(* deep enters also computational types (typ_rcd),
+   shallow only enters non-expansive types (bounds of path types, and/or-types) *)
+Inductive dmode: Set := deep | shallow.
+
+Inductive wf_typ: dmode -> ctx -> typ -> Prop :=
+  | wf_top: forall m G,
+      wf_typ m G typ_top
+  | wf_bot: forall m G,
+      wf_typ m G typ_bot
+  | wf_rcd_deep: forall G D,
+      wf_dec G D ->
+      wf_typ deep G (typ_rcd D)
+  | wf_rcd_shallow: forall G D,
+      wf_typ shallow G (typ_rcd D)
+  | wf_sel: forall m G x X L T U,
+      binds x X G ->
+      typ_has G X (dec_typ L T U) ->
+      (* Note: deep wf-ness of T and U was already checked at the definition site of x.L 
+      (wf_tmem), so it's sufficient to do a shallow check
+       --> allows x.L to appear recursively in T and U, but only behind a computational type
+       --> following upper bound terminates *)
+      wf_typ shallow G T ->
+      wf_typ shallow G U ->
+      wf_typ m G (typ_sel (avar_f x) L)
+  | wf_and: forall m G T1 T2,
+      wf_typ m G T1 ->
+      wf_typ m G T2 ->
+      wf_typ m G (typ_and T1 T2)
+  | wf_or: forall m G T1 T2,
+      wf_typ m G T1 ->
+      wf_typ m G T2 ->
+      wf_typ m G (typ_or T1 T2)
+(* wf_dec and wf_decs need no mode, because it's always deep *)
+with wf_dec: ctx -> dec -> Prop :=
+  | wf_tmem: forall G L Lo Hi,
+      wf_typ deep G Lo ->
+      wf_typ deep G Hi ->
+      wf_dec G (dec_typ L Lo Hi)
+  | wf_mtd: forall G m A R,
+      wf_typ deep G A ->
+      wf_typ deep G R ->
+      wf_dec G (dec_mtd m A R).
+
 Inductive subtyp: ctx -> typ -> typ -> Prop :=
   | subtyp_refl: forall G T,
+      wf_typ deep G T ->
       subtyp G T T
   | subtyp_top: forall G T,
+      wf_typ deep G T ->
       subtyp G T typ_top
   | subtyp_bot: forall G T,
+      wf_typ deep G T ->
       subtyp G typ_bot T
-  | subtyp_tdec: forall G L T1 U1 T2 U2,
-      subtyp G T2 T1 ->
-      subtyp G U1 U2 ->
-      subtyp G (typ_tdec L T1 U1) (typ_tdec L T2 U2)
-  | subtyp_mdec: forall G m T1 U1 T2 U2,
-      subtyp G T2 T1 ->
-      subtyp G U1 U2 ->
-      subtyp G (typ_mdec m T1 U1) (typ_mdec m T2 U2)
+  | subtyp_rcd: forall G D1 D2,
+      subdec G D1 D2 ->
+      subtyp G (typ_rcd D1) (typ_rcd D2)
   | subtyp_sel_l: forall G x X L T U,
       binds x X G ->
-      (*lookup_tdec fuel G X L = (T, U) ->*)
-      typ_has_tdec G X L T U ->
+      typ_has G X (dec_typ L T U) ->
       subtyp G T U -> (* <-- probably not needed, but keep for symmetry with subtyp_sel_r *)
       subtyp G (typ_sel (avar_f x) L) U
   | subtyp_sel_r: forall G x X L T U,
       binds x X G ->
-      (* lookup_tdec fuel G X L = (T, U) -> *)
-      typ_has_tdec G X L T U ->
+      typ_has G X (dec_typ L T U) ->
       subtyp G T U -> (* <-- makes proofs a lot easier!! *)
       subtyp G T (typ_sel (avar_f x) L)
   | subtyp_and: forall G T U1 U2,
@@ -224,55 +422,75 @@ Inductive subtyp: ctx -> typ -> typ -> Prop :=
       subtyp G T U2 ->
       subtyp G T (typ_and U1 U2)
   | subtyp_and_l: forall G T1 T2,
+      wf_typ deep G T1 ->
+      wf_typ deep G T2 ->
       subtyp G (typ_and T1 T2) T1
   | subtyp_and_r: forall G T1 T2,
+      wf_typ deep G T1 ->
+      wf_typ deep G T2 ->
       subtyp G (typ_and T1 T2) T2
   | subtyp_or: forall G T1 T2 U,
       subtyp G T1 U ->
       subtyp G T2 U ->
       subtyp G (typ_or T1 T2) U
   | subtyp_or_l: forall G T1 T2,
+      wf_typ deep G T1 ->
+      wf_typ deep G T2 ->
       subtyp G T1 (typ_or T1 T2)
   | subtyp_or_r: forall G T1 T2,
+      wf_typ deep G T1 ->
+      wf_typ deep G T2 ->
       subtyp G T2 (typ_or T1 T2)
   | subtyp_trans: forall G T1 T2 T3,
       subtyp G T1 T2 ->
       subtyp G T2 T3 ->
-      subtyp G T1 T3.
+      subtyp G T1 T3
+with subdec: ctx -> dec -> dec -> Prop :=
+  | subdec_typ: forall G L Lo1 Hi1 Lo2 Hi2,
+      subtyp G Lo2 Lo1 ->
+      subtyp G Hi1 Hi2 ->
+      subdec G (dec_typ L Lo1 Hi1) (dec_typ L Lo2 Hi2)
+  | subdec_mtd: forall m G S1 T1 S2 T2,
+      subtyp G S2 S1 ->
+      subtyp G T1 T2 ->
+      subdec G (dec_mtd m S1 T1) (dec_mtd m S2 T2).
 
 Inductive ty_trm: ctx -> trm -> typ -> Prop :=
   | ty_var: forall G x T,
       binds x T G ->
+      wf_typ deep G T ->
       ty_trm G (trm_var (avar_f x)) T
   | ty_call: forall G t T m U1 U2 V u,
       ty_trm G t T ->
-      (*lookup_mdec fuel G T m = Some (U2, V) ->*)
-      typ_has_mdec G T m U2 V ->
+      typ_has G T (dec_mtd m U2 V) ->
       ty_trm G u U1 ->
       subtyp G U1 U2 -> (* <-- explicit subsumption *)
+      wf_typ deep G V ->
       ty_trm G (trm_call t m u) V
   | ty_new: forall L G ds T u U,
       (forall x, x \notin L ->
          ty_defs (G & x ~ T) (open_defs x ds) T) ->
       (forall x, x \notin L ->
          ty_trm (G & x ~ T) (open_trm x u) U) ->
+      wf_typ deep G U -> (* <-- even stronger than x \notin fv_typ U *)
       ty_trm G (trm_new ds u) U
-with ty_def: ctx -> def -> typ -> Prop :=
+with ty_def: ctx -> def -> dec -> Prop :=
   | ty_tdef: forall G L T U,
       subtyp G T U -> (* <-- only allow realizable bounds *)
-      ty_def G (def_typ L T U) (typ_tdec L T U)
+      ty_def G (def_typ L T U) (dec_typ L T U)
   | ty_mdef: forall L m G T U1 U2 u,
+      wf_typ deep G T ->
       (forall x, x \notin L -> ty_trm (G & x ~ T) (open_trm x u) U1) ->
       subtyp G U1 U2 ->  (* <-- explicit subsumption *)
-      ty_def G (def_mtd m T U2 u) (typ_mdec m T U2)
+      ty_def G (def_mtd m T U2 u) (dec_mtd m T U2)
 with ty_defs: ctx -> defs -> typ -> Prop :=
   | ty_defs_nil: forall G,
       ty_defs G defs_nil typ_top
-  | ty_defs_cons: forall G ds d T1 T2,
-      ty_defs G ds T1 ->
-      ty_def G d T2 ->
+  | ty_defs_cons: forall G ds d T D,
+      ty_defs G ds T ->
+      ty_def G d D ->
       defs_hasnt ds (label_of_def d) -> (* <-- no duplicates *)
-      ty_defs G (defs_cons ds d) (typ_and T1 T2).
+      ty_defs G (defs_cons ds d) (typ_and T (typ_rcd D)).
 
 
 (** *** Well-formed store *)
@@ -312,10 +530,26 @@ Definition preservation := forall s G e T e' s',
 (* ###################################################################### *)
 (** ** Induction principles *)
 
+Scheme typ_mut := Induction for typ Sort Prop
+with   dec_mut := Induction for dec Sort Prop.
+Combined Scheme typ_mutind from typ_mut, dec_mut.
+
 Scheme trm_mut  := Induction for trm  Sort Prop
 with   def_mut  := Induction for def  Sort Prop
 with   defs_mut := Induction for defs Sort Prop.
 Combined Scheme trm_mutind from trm_mut, def_mut, defs_mut.
+
+Scheme typ_has_mut := Induction for typ_has Sort Prop
+with typ_hasnt_mut := Induction for typ_hasnt Sort Prop.
+Combined Scheme typ_has_mutind from typ_has_mut, typ_hasnt_mut.
+
+Scheme wf_typ_mut := Induction for wf_typ Sort Prop
+with   wf_dec_mut := Induction for wf_dec Sort Prop.
+Combined Scheme wf_mutind from wf_typ_mut, wf_dec_mut.
+
+Scheme subtyp_mut := Induction for subtyp Sort Prop
+with   subdec_mut := Induction for subdec Sort Prop.
+Combined Scheme subtyp_mutind from subtyp_mut, subdec_mut.
 
 Scheme ty_trm_mut    := Induction for ty_trm    Sort Prop
 with   ty_def_mut    := Induction for ty_def    Sort Prop
@@ -344,7 +578,12 @@ Ltac pick_fresh x :=
 Tactic Notation "apply_fresh" constr(T) "as" ident(x) :=
   apply_fresh_base T gather_vars x.
 
-Hint Constructors subtyp ty_trm ty_def ty_defs.
+Hint Constructors
+  typ_has typ_hasnt
+  wf_typ wf_dec
+  subtyp subdec
+  ty_trm ty_def ty_defs.
+Hint Constructors wf_sto.
 
 Lemma fresh_push_eq_inv: forall A x a (E: env A),
   x # (E & x ~ a) -> False.
@@ -373,11 +612,15 @@ Fixpoint subst_typ (z: var) (u: var) (T: typ) { struct T } : typ :=
   match T with
   | typ_top        => typ_top
   | typ_bot        => typ_bot
-  | typ_tdec L T U => typ_tdec L (subst_typ z u T) (subst_typ z u U)
-  | typ_mdec m T U => typ_mdec m (subst_typ z u T) (subst_typ z u U)
+  | typ_rcd D      => typ_rcd (subst_dec z u D)
   | typ_sel x L    => typ_sel (subst_avar z u x) L
   | typ_and T1 T2  => typ_and (subst_typ z u T1) (subst_typ z u T2)
   | typ_or  T1 T2  => typ_or  (subst_typ z u T1) (subst_typ z u T2)
+  end
+with subst_dec (z: var) (u: var) (D: dec) { struct D } : dec :=
+  match D with
+  | dec_typ L T U => dec_typ L (subst_typ z u T) (subst_typ z u U)
+  | dec_mtd m T U => dec_mtd m (subst_typ z u T) (subst_typ z u U)
   end.
 
 Fixpoint subst_trm (z: var) (u: var) (t: trm) : trm :=
@@ -409,10 +652,11 @@ Proof.
   intros. destruct* a. simpl. case_var*. simpls. notin_false.
 Qed.
 
-Lemma subst_fresh_typ: forall x y,
-  (forall T : typ , x \notin fv_typ  T  -> subst_typ  x y T  = T ).
+Lemma subst_fresh_typ_dec: forall x y,
+  (forall T : typ , x \notin fv_typ  T  -> subst_typ  x y T  = T ) /\
+  (forall D : dec , x \notin fv_dec  D  -> subst_dec  x y D  = D ).
 Proof.
-  intros x y T. induction T; intros; simpls; f_equal*. apply* subst_fresh_avar.
+  intros x y. apply typ_mutind; intros; simpls; f_equal*. apply* subst_fresh_avar.
 Qed.
 
 Lemma subst_fresh_trm_def_defs: forall x y,
@@ -421,7 +665,7 @@ Lemma subst_fresh_trm_def_defs: forall x y,
   (forall ds: defs, x \notin fv_defs ds -> subst_defs x y ds = ds).
 Proof.
   intros x y. apply trm_mutind; intros; simpls; f_equal*;
-    (apply* subst_fresh_avar || apply* subst_fresh_typ).
+    (apply* subst_fresh_avar || apply* subst_fresh_typ_dec).
 Qed.
 
 Lemma invert_fv_ctx_types_push: forall x z T G,
@@ -448,7 +692,7 @@ Proof.
     apply invert_fv_ctx_types_push in N. destruct N as [N1 N2].
     unfold subst_ctx in *. rewrite map_push.
     rewrite (IH N2).
-    rewrite (subst_fresh_typ _ _ N1).
+    rewrite ((proj1 (subst_fresh_typ_dec _ _)) _ N1).
     reflexivity.
 Qed.
 
@@ -465,12 +709,27 @@ Proof.
 Qed.
 
 (* "open and then substitute" = "substitute and then open" *)
-Lemma subst_open_commute_typ: forall x y u,
+Lemma subst_open_commute_typ_dec: forall x y u,
   (forall t : typ, forall n: nat,
      subst_typ x y (open_rec_typ n u t)
-     = open_rec_typ n (subst_fvar x y u) (subst_typ x y t)).
+     = open_rec_typ n (subst_fvar x y u) (subst_typ x y t)) /\
+  (forall D : dec, forall n: nat,
+     subst_dec x y (open_rec_dec n u D)
+     = open_rec_dec n (subst_fvar x y u) (subst_dec x y D)).
 Proof.
-  intros. induction t; intros; simpl; f_equal*. apply subst_open_commute_avar.
+  intros. apply typ_mutind; intros; simpl; f_equal*. apply subst_open_commute_avar.
+Qed.
+
+Lemma subst_open_commute_typ: forall x y u T,
+  subst_typ x y (open_typ u T) = open_typ (subst_fvar x y u) (subst_typ x y T).
+Proof.
+  intros. apply* subst_open_commute_typ_dec.
+Qed.
+
+Lemma subst_open_commute_dec: forall x y u D,
+  subst_dec x y (open_dec u D) = open_dec (subst_fvar x y u) (subst_dec x y D).
+Proof.
+  intros. apply* subst_open_commute_typ_dec.
 Qed.
 
 (* "open and then substitute" = "substitute and then open" *)
@@ -486,7 +745,7 @@ Lemma subst_open_commute_trm_def_defs: forall x y u,
      = open_rec_defs n (subst_fvar x y u) (subst_defs x y ds)).
 Proof.
   intros. apply trm_mutind; intros; simpl; f_equal*;
-    (apply* subst_open_commute_avar || apply* subst_open_commute_typ).
+    (apply* subst_open_commute_avar || apply* subst_open_commute_typ_dec).
 Qed.
 
 Lemma subst_open_commute_trm: forall x y u t,
@@ -523,7 +782,15 @@ Lemma subst_intro_typ: forall x u T, x \notin (fv_typ T) ->
   open_typ u T = subst_typ x u (open_typ x T).
 Proof.
   introv Fr. unfold open_typ. rewrite* subst_open_commute_typ.
-  lets Q: (@subst_fresh_typ x u). rewrite* (Q T).
+  destruct (@subst_fresh_typ_dec x u) as [Q _]. rewrite* (Q T).
+  unfold subst_fvar. case_var*.
+Qed.
+
+Lemma subst_intro_dec: forall x u D, x \notin (fv_dec D) ->
+  open_dec u D = subst_dec x u (open_dec x D).
+Proof.
+  introv Fr. unfold open_trm. rewrite* subst_open_commute_dec.
+  destruct (@subst_fresh_typ_dec x u) as [_ Q]. rewrite* (Q D).
   unfold subst_fvar. case_var*.
 Qed.
 
@@ -535,11 +802,12 @@ Proof.
   + unfold fv_avar in H. assert (y <> v) by auto. repeat case_if; reflexivity.
 Qed.
 
-Lemma subst_undo_typ: forall x y,
-   (forall T , y \notin fv_typ  T  -> (subst_typ  y x (subst_typ  x y T )) = T ).
+Lemma subst_undo_typ_dec: forall x y,
+   (forall T , y \notin fv_typ  T  -> (subst_typ  y x (subst_typ  x y T )) = T )
+/\ (forall D , y \notin fv_dec  D  -> (subst_dec  y x (subst_dec  x y D )) = D ).
 Proof.
   intros.
-  induction T; intros; simpl; unfold fv_typ in *; f_equal*.
+  apply typ_mutind; intros; simpl; unfold fv_typ, fv_dec in *; f_equal*.
   apply* subst_undo_avar.
 Qed.
 
@@ -550,14 +818,95 @@ Lemma subst_undo_trm_def_defs: forall x y,
 Proof.
   intros.
   apply trm_mutind; intros; simpl; unfold fv_trm, fv_def, fv_defs in *; f_equal*;
-    (apply* subst_undo_avar || apply* subst_undo_typ).
+    (apply* subst_undo_avar || apply* subst_undo_typ_dec).
 Qed.
 
-Lemma subst_undo_trm: forall x y t,
+Lemma subst_typ_undo: forall x y T,
+  y \notin fv_typ T -> (subst_typ y x (subst_typ x y T)) = T.
+Proof.
+  apply* subst_undo_typ_dec.
+Qed.
+
+Lemma subst_trm_undo: forall x y t,
   y \notin fv_trm t -> (subst_trm y x (subst_trm x y t)) = t.
 Proof.
   apply* subst_undo_trm_def_defs.
 Qed.
+
+
+(* ###################################################################### *)
+(** ** Regularity of Typing *)
+
+Lemma wf_deep_to_any: forall m G T,
+  wf_typ deep G T ->
+  wf_typ m G T.
+Proof.
+  introv WfT. gen_eq m20: deep. induction WfT; intro Eq; subst; destruct m; eauto.
+  discriminate.
+Qed.
+
+Hint Resolve wf_deep_to_any.
+
+(* If a type is involved in a subtyping judgment, it is (deeply) well-formed. *)
+Lemma subtyping_regular:
+   (forall G T1 T2, subtyp G T1 T2 -> wf_typ deep G T1 /\ wf_typ deep G T2)
+/\ (forall G D1 D2, subdec G D1 D2 -> wf_dec      G D1 /\ wf_dec      G D2).
+Proof.
+  apply subtyp_mutind; intros; split; subst;
+  repeat match goal with
+  | H: _ /\ _ |- _ => destruct H
+  | H: wf_dec _ (dec_typ _ _ _) |- _ => inversions H
+  | H: wf_dec _ (dec_mtd _ _ _) |- _ => inversions H
+  end;
+  eauto.
+Qed.
+
+Definition subtyp_regular := proj1 subtyping_regular.
+Definition subdec_regular := proj2 subtyping_regular.
+
+Lemma strengthen_wf:
+   (forall m G T, wf_typ m G T -> forall G1 x U G2,
+    G = G1 & x ~ U & G2 ->
+    x \notin fv_typ T ->
+    wf_typ m (G1 & G2) T)
+/\ (forall G D, wf_dec G D -> forall G1 x U G2,
+    G = G1 & x ~ U & G2 ->
+    x \notin fv_dec D ->
+    wf_dec (G1 & G2) D).
+Proof.
+  apply wf_mutind.
+  + (* case wf_top *) eauto.
+  + (* case wf_bot *) eauto.
+  + (* case wf_rcd_deep *) eauto.
+  + (* case wf_rcd_shallow *) eauto.
+  + (* case wf_sel *)
+    introv Bi Has WfT IHT WfU IHU Eq N. subst.
+    specialize (IHT _ _ _ _ eq_refl).
+    specialize (IHU _ _ _ _ eq_refl).
+    (* Does not hold because x0 \notin x.L does not imply x0 \notin T, U *)
+Abort.
+
+Lemma typing_regular:
+   (forall G t T, ty_trm G t T ->
+      wf_typ deep G T)
+/\ (forall G d D, ty_def G d D ->
+      wf_dec G D)
+/\ (forall G ds T, ty_defs G ds T ->
+      wf_typ deep G T).
+Proof.
+  apply ty_mutind; intros; subst;
+  repeat match goal with
+  | H: _ /\ _ |- _ => destruct H
+  | H: wf_dec _ (dec_typ _ _ _) |- _ => inversions H
+  | H: wf_dec _ (dec_mtd _ _ _) |- _ => inversions H
+  | H: subtyp _ _ _ |- _ => apply subtyp_regular in H
+  end;
+  eauto.
+Qed.
+
+Definition ty_trm_regular  := proj1        typing_regular.
+Definition ty_def_regular  := proj1 (proj2 typing_regular).
+Definition ty_defs_regular := proj2 (proj2 typing_regular).
 
 
 (* ###################################################################### *)
@@ -571,8 +920,708 @@ Admitted.
 
 
 (* ###################################################################### *)
+(** ** More stuff *)
+
+Lemma intersect_dec_total: forall D1 D2,
+  label_of_dec D1 = label_of_dec D2 ->
+  exists D12, D1 && D2 == D12.
+Proof.
+  introv Eq.
+  destruct D1; destruct D2; inversions Eq; unfold intersect_dec; simpl; case_if; eauto.
+Qed.
+
+Lemma union_dec_total: forall D1 D2,
+  label_of_dec D1 = label_of_dec D2 ->
+  exists D12, D1 || D2 == D12.
+Proof.
+  introv Eq.
+  destruct D1; destruct D2; inversions Eq; unfold union_dec; simpl; case_if; eauto.
+Qed.
+
+Lemma intersect_dec_label_eq: forall D1 D2 D12,
+  D1 && D2 == D12 ->
+  label_of_dec D1 = label_of_dec D2 /\
+  label_of_dec D1 = label_of_dec D12 /\
+  label_of_dec D2 = label_of_dec D12.
+Proof.
+  intros. destruct D1; destruct D2; unfold intersect_dec in H; simpl; case_if; 
+  inversions H; auto.
+Qed.
+
+Lemma union_dec_label_eq: forall D1 D2 D12,
+  D1 || D2 == D12 ->
+  label_of_dec D1 = label_of_dec D2 /\
+  label_of_dec D1 = label_of_dec D12 /\
+  label_of_dec D2 = label_of_dec D12.
+Proof.
+  intros. destruct D1; destruct D2; unfold union_dec in H; simpl; case_if; 
+  inversions H; auto.
+Qed.
+
+Lemma subdec_to_label_of_dec_eq: forall G D1 D2,
+  subdec G D1 D2 -> label_of_dec D1 = label_of_dec D2.
+Proof.
+  introv Sd. inversions Sd; reflexivity.
+Qed.
+
+Lemma invert_subdec_typ_sync_left: forall G D L Lo2 Hi2,
+   subdec G D (dec_typ L Lo2 Hi2) ->
+   exists Lo1 Hi1, D = (dec_typ L Lo1 Hi1) /\
+                   subtyp G Lo2 Lo1 /\
+                   subtyp G Hi1 Hi2.
+Proof.
+  introv Sd. inversions Sd. exists Lo1 Hi1. auto.
+Qed.
+
+Lemma invert_subdec_mtd_sync_left: forall G D m T2 U2,
+   subdec G D (dec_mtd m T2 U2) ->
+   exists T1 U1, D = (dec_mtd m T1 U1) /\
+                 subtyp G T2 T1 /\
+                 subtyp G U1 U2.
+Proof.
+  introv Sd. inversions Sd. exists S1 T1. auto.
+Qed.
+
+
+(* ###################################################################### *)
+(** ** typ_has/hasnt total *)
+
+Lemma typ_has_total: forall m G T, wf_typ m G T ->
+  forall l, typ_hasnt G T l \/ exists D, l = label_of_dec D /\ typ_has G T D.
+Proof.
+  introv Wf. induction Wf; intro l.
+  + (* case wf_top *)
+    left. apply typ_top_hasnt.
+  + (* case wf_bot *)
+    right. exists (dec_bot l). split.
+    - destruct l; reflexivity.
+    - apply typ_bot_has.
+  + (* case wf_rcd_deep *)
+    destruct (classicT (l = label_of_dec D)) as [Eq | Ne].
+    - right. exists D. split.
+      * apply Eq.
+      * apply typ_rcd_has.
+    - left. apply (typ_rcd_hasnt _ _ Ne).
+  + (* case wf_rcd_shallow  *)
+    destruct (classicT (l = label_of_dec D)) as [Eq | Ne].
+    - right. exists D. split.
+      * apply Eq.
+      * apply typ_rcd_has.
+    - left. apply (typ_rcd_hasnt _ _ Ne).
+  + (* case wf_sel *)
+    specialize (IHWf2 l). destruct IHWf2 as [UHasnt | [D [Eq UHas]]].
+    - left. apply (typ_sel_hasnt H H0 UHasnt).
+    - right. exists D. split.
+      * apply Eq.
+      * apply (typ_sel_has H H0 UHas).
+  + (* case wf_and *)
+    specialize (IHWf1 l). specialize (IHWf2 l).
+    destruct IHWf1 as [T1Hasnt | [D1 [Eq1 T1Has]]];
+    destruct IHWf2 as [T2Hasnt | [D2 [Eq2 T2Has]]].
+    - left. apply (typ_and_hasnt T1Hasnt T2Hasnt).
+    - right. exists D2. apply (conj Eq2).
+      rewrite Eq2 in T1Hasnt. apply (typ_and_has_2 T1Hasnt T2Has).
+    - right. exists D1. apply (conj Eq1).
+      rewrite Eq1 in T2Hasnt. apply (typ_and_has_1 T1Has T2Hasnt).
+    - right.
+      lets Eq12: Eq2. rewrite Eq1 in Eq12.
+      destruct (intersect_dec_total D1 D2 Eq12) as [D12 Eq].
+      exists D12. rewrite Eq1.
+      apply (conj (proj32 (intersect_dec_label_eq _ _ Eq))).
+      apply (typ_and_has_12 T1Has T2Has Eq).
+  + (* case wf_or *)
+    specialize (IHWf1 l). specialize (IHWf2 l).
+    destruct IHWf1 as [T1Hasnt | [D1 [Eq1 T1Has]]];
+    destruct IHWf2 as [T2Hasnt | [D2 [Eq2 T2Has]]].
+    - left. apply (typ_or_hasnt_1 _ T1Hasnt).
+    - left. apply (typ_or_hasnt_1 _ T1Hasnt).
+    - left. apply (typ_or_hasnt_2 _ T2Hasnt).
+    - right.
+      lets Eq12: Eq2. rewrite Eq1 in Eq12.
+      destruct (union_dec_total D1 D2 Eq12) as [D12 Eq].
+      exists D12. rewrite Eq1.
+      apply (conj (proj32 (union_dec_label_eq _ _ Eq))).
+      apply (typ_or_has T1Has T2Has Eq).
+Qed.
+
+Print Assumptions typ_has_total.
+
+
+(* ###################################################################### *)
+(** ** Uniqueness *)
+
+Lemma intersect_dec_unique: forall D1 D2 D3 D4,
+  D1 && D2 == D3 ->
+  D1 && D2 == D4 ->
+  D3 = D4.
+Proof.
+  introv Eq3 Eq4. rewrite Eq3 in Eq4. inversions Eq4. reflexivity.
+Qed.
+
+Lemma union_dec_unique: forall D1 D2 D3 D4,
+  D1 || D2 == D3 ->
+  D1 || D2 == D4 ->
+  D3 = D4.
+Proof.
+  introv Eq3 Eq4. rewrite Eq3 in Eq4. inversions Eq4. reflexivity.
+Qed.
+
+(* need to prove the same things several times to make sure we always have an IH *)
+Lemma typ_has_unique_and_not_hasnt:
+   (forall G T D1, typ_has G T D1 ->
+        (forall D2, typ_has G T D2 -> label_of_dec D1 = label_of_dec D2 -> D1 = D2)
+     /\ (typ_hasnt G T (label_of_dec D1) -> False))
+/\ (forall G T l, typ_hasnt G T l ->
+      forall D, l = label_of_dec D -> typ_has G T D -> False).
+Proof.
+  apply typ_has_mutind; try split.
+  + (* case typ_bot_has *)
+    introv Has Eq. inversions Has; simpl in Eq; try discriminate.
+    destruct l; destruct l0; simpl in *; inversions Eq; reflexivity.
+  + (* case typ_bot_has *)
+    introv Hasnt. inversions Hasnt.
+  + (* case typ_rcd_has *)
+    introv Has Eq. inversions Has. reflexivity.
+  + (* case typ_rcd_has *)
+    introv Hasnt. inversions Hasnt. apply H1. reflexivity.
+  + (* case typ_sel_has *)
+    rename b into Bi, t into THas, H into IH1, t0 into HiHas, H0 into IH2.
+    introv Has' Eq.
+    inversions Has'. rename T0 into T', H1 into Bi', H3 into THas', H5 into HiHas'.
+    lets EqT: (binds_func Bi' Bi). subst T'. clear Bi'.
+    destruct IH1 as [IH1 _]. destruct IH2 as [IH2 _].
+    specialize (IH1 _ THas' eq_refl). symmetry in IH1. inversions IH1.
+    apply (IH2 _ HiHas' Eq).
+  + (* case typ_sel_has *)
+    rename b into Bi, t into THas, H into IH1, t0 into HiHas, H0 into IH2.
+    introv Hasnt.
+    destruct IH2 as [_ IH2]. inversions Hasnt.
+    rename T0 into T', H1 into Bi', H3 into THas', H5 into HiHasnt.
+    lets EqT: (binds_func Bi' Bi). subst T'. clear Bi'.
+    destruct IH1 as [IH1 _]. specialize (IH1 _ THas' eq_refl).
+    symmetry in IH1. inversions IH1. apply (IH2 HiHasnt).
+  + (* case typ_and_has_1 *)
+    rename t into T1Has, H into IH1, t0 into T2Hasnt, H0 into IH2.
+    introv Has' Eq. destruct IH1 as [IH1 _].
+    inversions Has'.
+    - eauto.
+    - exfalso. apply (IH2 _ Eq H4).
+    - exfalso. refine (IH2 _ _ H3).
+      rewrite Eq. symmetry. apply (proj33 (intersect_dec_label_eq _ _ H5)).
+  + (* case typ_and_has_1 *)
+    rename t into T1Has, H into IH1, t0 into T2Has, H0 into IH2.
+    introv T12Hasnt. inversions T12Hasnt. destruct IH1 as [_ IH1]. apply (IH1 H2).
+  + (* case typ_and_has_2 *)
+    rename t into T1Hasnt, H into IH1, t0 into T2Has, H0 into IH2.
+    introv Has' Eq. destruct IH2 as [IH2 _].
+    inversions Has'.
+    - exfalso. refine (IH1 _ Eq H2).
+    - eauto.
+    - exfalso. refine (IH1 _ _ H1).
+      rewrite Eq. symmetry. apply (proj32 (intersect_dec_label_eq _ _ H5)).
+  + (* case typ_and_has_2 *)
+    rename t into T1Hasnt, H into IH1, t0 into T2Has, H0 into IH2.
+    introv T12Hasnt. inversions T12Hasnt. destruct IH2 as [_ IH2]. apply (IH2 H4).
+  + (* case typ_and_has_12 *)
+    rename t into T1Has, H into IH1, t0 into T2Has, H0 into IH2.
+    introv Has' Eq.
+    remember (label_of_dec D0) as l eqn: Eq0.
+    symmetry in Eq. rename Eq into Eq3.
+    destruct (intersect_dec_label_eq _ _ e) as [Eq12 [Eq13 Eq23]].
+    rewrite <- Eq3 in Eq23. symmetry in Eq23; rename Eq23 into Eq2.
+    rewrite <- Eq3 in Eq13. symmetry in Eq13; rename Eq13 into Eq1. clear Eq12.
+    lets Eq: (conj Eq0 (conj Eq1 (conj Eq2 Eq3))). clear Eq0 Eq1 Eq2 Eq3.
+    inversions Has'.
+    - exfalso. rewrite <- (proj41 Eq) in H4. rewrite (proj43 Eq) in H4.
+      destruct IH2 as [_ IH2]. apply (IH2 H4).
+    - exfalso. rewrite <- (proj41 Eq) in H2. rewrite (proj42 Eq) in H2.
+      destruct IH1 as [_ IH1]. apply (IH1 H2).
+    - destruct (intersect_dec_label_eq _ _ H5) as [Eq45 [Eq40 Eq50]].
+      destruct IH1 as [IH1 _]. specialize (IH1 D4).
+      rewrite Eq40 in IH1. rewrite <- (proj41 Eq) in IH1. rewrite <- (proj42 Eq) in IH1.
+      specialize (IH1 H1 eq_refl). subst D4.
+      destruct IH2 as [IH2 _]. specialize (IH2 D5).
+      rewrite Eq50 in IH2. rewrite <- (proj41 Eq) in IH2. rewrite <- (proj43 Eq) in IH2.
+      specialize (IH2 H3 eq_refl). subst D5.
+      apply (intersect_dec_unique _ _ e H5).
+  + (* case typ_and_has_12 *)
+    rename t into T1Hasnt, H into IH1, t0 into T2Has, H0 into IH2.
+    introv T12Hasnt. inversions T12Hasnt. destruct IH2 as [_ IH2].
+    destruct (intersect_dec_label_eq _ _ e) as [Eq12 [Eq13 Eq23]].
+    rewrite Eq23 in IH2. apply (IH2 H4).
+  + (* case typ_or_has *)
+    rename t into T1Has, H into IH1, t0 into T2Has, H0 into IH2.
+    introv T12Has Eq. inversions T12Has.
+    remember (label_of_dec D0) as l eqn: Eq0.
+    symmetry in Eq. rename Eq into Eq3.
+    destruct (union_dec_label_eq _ _ e) as [Eq12 [Eq13 Eq23]].
+    destruct (union_dec_label_eq _ _ H5) as [Eq45 [Eq40 Eq50]].
+    destruct IH1 as [IH1 _]. specialize (IH1 D4).
+    rewrite Eq40 in IH1. rewrite <- Eq0 in IH1. rewrite Eq3 in IH1.
+    specialize (IH1 H1 Eq13). subst D4.
+    destruct IH2 as [IH2 _]. specialize (IH2 D5).
+    rewrite Eq50 in IH2. rewrite <- Eq0 in IH2. rewrite Eq3 in IH2.
+    specialize (IH2 H3 Eq23). subst D5.
+    apply (union_dec_unique _ _ e H5).
+  + (* case typ_or_has *)
+    rename t into T1Has, H into IH1, t0 into T2Has, H0 into IH2.
+    destruct (union_dec_label_eq _ _ e) as [Eq12 [Eq13 Eq23]].
+    introv T12Hasnt. inversions T12Hasnt.
+    - destruct IH1 as [_ IH1].
+      rewrite Eq13 in IH1. apply (IH1 H3).
+    - destruct IH2 as [_ IH2].
+      rewrite Eq23 in IH2. apply (IH2 H3).
+  + (* case typ_top_hasnt *)
+    introv Eq Has. inversions Has.
+  + (* case typ_rcd_hasnt *)
+    introv Ne Eq Has. inversions Has. apply Ne. reflexivity.
+  + (* case typ_sel_hasnt *)
+    introv Bi THas IH1 HiHasnt IH2 Eq Has'.
+    inversions Has'. rename T0 into T', H1 into Bi', H3 into THas', H5 into HiHas.
+    lets EqT: (binds_func Bi' Bi). subst T'. clear Bi'.
+    destruct IH1 as [IH1 _]. specialize (IH1 _ THas' eq_refl).
+    symmetry in IH1. inversions IH1. apply (IH2 _ eq_refl HiHas).
+  + (* case typ_and_hasnt *)
+    introv T1Hasnt IH1 T2Hasnt IH2 Eq Has'.
+    inversions Has'.
+    - eauto.
+    - eauto.
+    - destruct (intersect_dec_label_eq _ _ H5) as [Eq12 [Eq1 Eq2]].
+      rewrite <- Eq1 in *. apply (IH1 _ eq_refl H1).
+  + (* case typ_or_hasnt_1 *)
+    introv T1Hasnt IH Eq Has'. inversions Has'.
+    destruct (union_dec_label_eq _ _ H5) as [Eq12 [Eq1 Eq2]].
+    rewrite <- Eq1 in *. apply (IH _ eq_refl H1).
+  + (* case typ_or_hasnt_2 *)
+    introv T2Hasnt IH Eq Has'. inversions Has'.
+    destruct (union_dec_label_eq _ _ H5) as [Eq12 [Eq1 Eq2]].
+    rewrite <- Eq2 in *. apply (IH _ eq_refl H3).
+Qed.
+
+Print Assumptions typ_has_unique_and_not_hasnt.
+
+Lemma typ_has_unique: forall G T D1 D2,
+  typ_has G T D1 ->
+  typ_has G T D2 ->
+  label_of_dec D1 = label_of_dec D2 ->
+  D1 = D2.
+Proof.
+  introv H1 H2 Eq.
+  destruct typ_has_unique_and_not_hasnt as [P _].
+  specialize (P G T D1 H1). destruct P as [P _]. apply (P _ H2 Eq).
+Qed.
+
+Lemma not_typ_has_and_hasnt: forall G T D,
+  typ_has G T D -> typ_hasnt G T (label_of_dec D) -> False.
+Proof.
+  introv Has Hasnt.
+  destruct typ_has_unique_and_not_hasnt as [_ P].
+  apply (P G T (label_of_dec D) Hasnt D eq_refl Has).
+Qed.
+
+
+(* ###################################################################### *)
+(** ** Looks like rules, but follows from the rules *)
+
+(* take subtyp_and/or rules and replace "and" by "intersect", "or" by "union": *)
+
+Lemma subtyp_intersect : forall (G : ctx) (S T1 T2 : typ),
+  subtyp G S T1 -> subtyp G S T2 -> subtyp G S (intersect_typ T1 T2).
+Proof.
+  intros. destruct T1; destruct T2; unfold intersect_typ; case_if; simpl; auto.
+Qed.
+
+(*
+Lemma subtyp_intersect_l : forall (G : ctx) (T1 T2 S : typ),
+  subtyp G T1 S ->
+  subtyp G (intersect_typ T1 T2) S.
+Proof.
+  intros. destruct (subtyp_regular H) as [WfT1 WfS].
+  destruct T1; destruct T2; destruct S; simpl; unfold intersect_typ; case_if; auto.
+  refine (subtyp_trans (subtyp_top _) H); auto.
+Qed.
+
+Lemma subtyp_intersect_r : forall (G : ctx) (T1 T2 S : typ),
+  subtyp G T2 S -> subtyp G (intersect_typ T1 T2) S.
+Proof.
+  intros.
+  destruct T1; destruct T2; destruct S; simpl; auto;
+  apply (subtyp_trans (subtyp_top _ _) H).
+Qed.
+*)
+
+Lemma subtyp_union : forall (G : ctx) (T1 T2 S : typ),
+  subtyp G T1 S -> subtyp G T2 S -> subtyp G (union_typ T1 T2) S.
+Proof.
+  intros.
+  destruct T1; destruct T2; destruct S; unfold union_typ; case_if; simpl; auto.
+Qed.
+
+(*
+Lemma subtyp_union_l : forall (G : ctx) (S T1 T2 : typ),
+  subtyp G S T1 -> subtyp G S (union_typ T1 T2).
+Proof.
+  intros.
+  destruct T1; destruct T2; destruct S; simpl; auto;
+  apply (subtyp_trans H (subtyp_bot _ _)).
+Qed.
+
+Lemma subtyp_union_r: forall (G : ctx) (S T1 T2 : typ),
+  subtyp G S T2 -> subtyp G S (union_typ T1 T2).
+Proof.
+  intros.
+  destruct T1; destruct T2; destruct S; simpl; auto;
+  apply (subtyp_trans H (subtyp_bot _ _)).
+Qed.
+
+Hint Resolve subtyp_intersect subtyp_intersect_l subtyp_intersect_r
+             subtyp_union     subtyp_union_l     subtyp_union_r.
+*)
+
+Hint Resolve subtyp_intersect subtyp_union.
+
+Lemma subdec_intersect: forall G D0 D1 D2 D12,
+  subdec G D0 D1 ->
+  subdec G D0 D2 ->
+  D1 && D2 == D12 ->
+  subdec G D0 D12.
+Proof.
+  introv Sd01 Sd02 I. inversions Sd01; inversions Sd02;
+  unfold intersect_dec in I; case_if; inversions I; auto.
+Qed.
+
+Lemma subdec_union: forall G D D1 D2 D12,
+  subdec G D1 D ->
+  subdec G D2 D ->
+  D1 || D2 == D12 ->
+  subdec G D12 D.
+Proof.
+  introv Sd01 Sd02 I. inversions Sd01; inversions Sd02;
+  unfold union_dec in I; case_if; inversions I; auto.
+Qed.
+
+Lemma subdec_intersect_l: forall G D1 D2 D12,
+  D1 && D2 == D12 ->
+  wf_dec G D1 ->
+  wf_dec G D12 ->
+  subdec G D12 D1.
+Admitted.
+
+Lemma subdec_union_l: forall G D0 D1 D2 D12,
+  subdec G D0 D1 ->
+  D1 || D2 == D12 ->
+  wf_dec G D2 ->
+  subdec G D0 D12.
+Admitted. (*
+Proof.
+  introv Sd I Wf2. inversions Sd; destruct D2;
+  unfold union_dec in I; case_if; inversions I; simpl in *; inversions H1;
+  inversions Wf2.
+  - destruct (subtyp_regular H) as [WfLo2 WfLo1].
+    destruct (subtyp_regular H0) as [WfHi1 WfHi2].
+    apply subdec_typ.
+    * apply (subtyp_trans (subtyp_and_l WfLo2 H4) H).
+    * refine (subtyp_trans H0 (subtyp_or_l WfHi2 H6)).
+ - destruct (subtyp_regular H) as [WfLo2 WfLo1].
+   destruct (subtyp_regular H0) as [WfHi1 WfHi2].
+    apply subdec_mtd.
+    * apply (subtyp_trans (subtyp_and_l WfLo2 H4) H).
+    * refine (subtyp_trans H0 (subtyp_or_l WfHi2 H6)).
+Qed.
+
+Lemma subdec_union_r: forall G D0 D1 D2 D12,
+  subdec G D0 D2 ->
+  D1 || D2 == D12 ->
+  wf_dec G D1 ->
+  subdec G D0 D12.
+Proof.
+  introv Sd I Wf2. inversions Sd; destruct D1;
+  unfold union_dec in I; case_if; inversions I; simpl in *; inversions H1;
+  inversions Wf2.
+  - destruct (subtyp_regular H) as [WfLo2 WfLo1].
+    destruct (subtyp_regular H0) as [WfHi1 WfHi2].
+    apply subdec_typ.
+    * refine (subtyp_trans (subtyp_and_r H4 WfLo2) H).
+    * refine (subtyp_trans H0 (subtyp_or_r H6 WfHi2)).
+ - destruct (subtyp_regular H) as [WfLo2 WfLo1].
+   destruct (subtyp_regular H0) as [WfHi1 WfHi2].
+    apply subdec_mtd.
+    * refine (subtyp_trans (subtyp_and_r H4 WfLo2) H).
+    * refine (subtyp_trans H0 (subtyp_or_r H6 WfHi2)).
+Qed.
+*)
+
+
+(* ###################################################################### *)
 (** ** subtyp-and-then-lookup_tdec to lookup_tdec-and-then-subdec *)
 
+Lemma typ_has_preserves_wf: forall G T D,
+  typ_has G T D ->
+  wf_typ deep G T ->
+  wf_dec G D.
+Proof.
+  introv Has. induction Has; introv Wf.
+  + (* case typ_bot_has *)
+    destruct l; simpl; eauto.
+  + (* case typ_rcd_has *)
+    inversions Wf. eauto.
+  + (* case typ_sel_has *)
+    inversions Wf. lets Eq: (binds_func H H2). subst T.
+    assert (WfX: wf_typ deep G X) by admit. (* <-- doesn't hold !!! *)
+    apply IHHas2.
+    specialize (IHHas1 WfX). inversions IHHas1. assumption.
+  + (* case typ_and_has_1 *)
+    inversions Wf. eauto.
+  + (* case typ_and_has_2 *)
+    inversions Wf. eauto.
+  + (* case typ_and_has_12 *)
+    inversions Wf. admit. (* TODO *)
+  + (* case typ_or_has *)
+    admit. (* TODO *)
+Abort.
+
+Lemma subdec2_to_label_of_dec_eq: forall G D1 D2,
+  subdec G D1 D2 \/ D1 = D2 \/ D1 = dec_bot (label_of_dec D2) ->
+  label_of_dec D1 = label_of_dec D2.
+Proof.
+  introv H. destruct H as [Sd | [Eq | Eq]].
+  - apply (subdec_to_label_of_dec_eq Sd).
+  - subst. reflexivity.
+  - rewrite Eq. destruct D2; reflexivity.
+Qed.
+
+Lemma subdec_trans: forall G D1 D2 D3,
+  subdec G D1 D2 -> subdec G D2 D3 -> subdec G D1 D3.
+Proof.
+  introv H12 H23. inversions H12; inversions H23; constructor;
+  solve [ assumption | (eapply subtyp_trans; eassumption)].
+Qed.
+
+Lemma subdec2_trans: forall G D1 D2 D3,
+  subdec G D1 D2 \/ D1 = D2 \/ D1 = dec_bot (label_of_dec D2) ->
+  subdec G D2 D3 \/ D2 = D3 \/ D2 = dec_bot (label_of_dec D3) ->
+  subdec G D1 D3 \/ D1 = D3 \/ D1 = dec_bot (label_of_dec D3).
+Proof.
+  introv H12 H23.
+  destruct H12 as [H12 | [H12 | H12]]; destruct H23 as [H23 | [H23 | H23]];
+  try solve [subst; auto].
+  - left. apply (subdec_trans H12 H23).
+  - (* oooops... doesn't hold ! *)
+Abort.
+
+Lemma intersect_dec_refl: forall D D2, D && D == D2 -> D = D2.
+Proof.
+  intros. unfold intersect_dec in H. case_if in H.
+  destruct D as [L S1 U1 | m S1 U1]; inversions H; unfold union_typ; unfold intersect_typ;
+  case_if; case_if; reflexivity.
+Qed.
+
+Lemma union_dec_refl: forall D D2, D || D == D2 -> D = D2.
+Proof.
+  intros. unfold union_dec in H. case_if in H.
+  destruct D as [L S1 U1 | m S1 U1]; inversions H; unfold union_typ; unfold intersect_typ;
+  case_if; case_if; reflexivity.
+Qed.
+
+Lemma subdec2_intersect: forall G D0 D1 D2 D12,
+  subdec G D0 D1 \/ D0 = D1 \/ D0 = dec_bot (label_of_dec D1) ->
+  subdec G D0 D2 \/ D0 = D2 \/ D0 = dec_bot (label_of_dec D2) ->
+  D1 && D2 == D12 ->
+  subdec G D0 D12 \/ D0 = D12 \/ D0 = dec_bot (label_of_dec D12).
+Proof.
+  introv Sd1 Sd2 Eq.
+  destruct (intersect_dec_label_eq _ _ Eq) as [Eq12 [Eq112 Eq212]].
+  destruct Sd1 as [Sd1 | [Sd1 | Sd1]]; destruct Sd2 as [Sd2 | [Sd2 | Sd2]].
+  - left. apply (subdec_intersect Sd1 Sd2 Eq).
+  - subst D2. left. inversions Sd1.
+    * destruct D12 as [L' Lo12 Hi12 | ]; unfold intersect_dec in Eq; case_if; inversions Eq.
+      apply subdec_typ.
+      + apply (subtyp_union H).
+        destruct (subtyp_regular H) as [_ Wf]. apply (subtyp_refl Wf).
+      + apply (subtyp_intersect H0).
+        destruct (subtyp_regular H0) as [Wf _]. apply (subtyp_refl Wf).
+    * destruct D12 as [| m' A R]; unfold intersect_dec in Eq; case_if; inversions Eq.
+      apply subdec_mtd.
+      + apply (subtyp_union H).
+        destruct (subtyp_regular H) as [_ Wf]. apply (subtyp_refl Wf).
+      + apply (subtyp_intersect H0).
+        destruct (subtyp_regular H0) as [Wf _]. apply (subtyp_refl Wf).
+  - rewrite Eq212 in Sd2. right. right. exact Sd2.
+  - subst D0. left. inversions Sd2.
+    * destruct D12 as [L' Lo12 Hi12 | ]; unfold intersect_dec in Eq; case_if; inversions Eq.
+      apply subdec_typ.
+      + refine (subtyp_union _ H).
+        destruct (subtyp_regular H) as [_ Wf]. apply (subtyp_refl Wf).
+      + refine (subtyp_intersect _ H0).
+        destruct (subtyp_regular H0) as [Wf _]. apply (subtyp_refl Wf).
+    * destruct D12 as [| m' A R]; unfold intersect_dec in Eq; case_if; inversions Eq.
+      apply subdec_mtd.
+      + refine (subtyp_union _ H).
+        destruct (subtyp_regular H) as [_ Wf]. apply (subtyp_refl Wf).
+      + refine (subtyp_intersect _ H0).
+        destruct (subtyp_regular H0) as [Wf _]. apply (subtyp_refl Wf).
+  - subst D0. subst D1. apply intersect_dec_refl in Eq. auto.
+  - subst D0. rewrite Eq212 in Sd2. auto.
+  - subst D0. rewrite Eq112. auto.
+  - subst D0. rewrite Eq112. auto.
+  - subst D0. rewrite Eq112. auto.
+Qed.
+
+Print Assumptions subdec2_intersect.
+
+Lemma swap_sub_and_typ_has: forall G T1 T2 D2,
+  subtyp G T1 T2 ->
+  typ_has G T2 D2 ->
+  exists D1,
+    typ_has G T1 D1 /\
+    (subdec G D1 D2 \/ D1 = D2 \/ D1 = dec_bot (label_of_dec D2)).
+Proof.
+  introv St. gen D2. induction St; introv T2Has.
+  + (* case subtyp_refl *)
+    eexists. apply (conj T2Has). auto.
+  + (* case subtyp_top *)
+    inversions T2Has.
+  + (* case subtyp_bot *)
+    rename T into T2.
+    exists (dec_bot (label_of_dec D2)). split.
+    - auto.
+    - right. right. reflexivity.
+  + (* case subtyp_rcd *)
+    inversions T2Has. rename D0 into D2. exists D1. auto.
+  + (* case subtyp_sel_l *)
+    rename H into Bi, H0 into XHas.
+    exists D2. eauto.
+  + (* case subtyp_sel_r *)
+    rename H into Bi, H0 into XHas.
+    inversions T2Has.
+    lets Eq: (binds_func H1 Bi). subst T0.
+    apply IHSt. clear IHSt.
+    lets Eq: (typ_has_unique H3 XHas eq_refl). inversions Eq.
+    exact H5.
+  + (* case subtyp_and *)
+    inversions T2Has.
+    - eauto.
+    - eauto.
+    - rename H1 into U1Has, H3 into U2Has, H5 into Eq, D1 into DU1, D0 into DU2.
+      specialize (IHSt1 _ U1Has). destruct IHSt1 as [D1 [THas Sd1]].
+      specialize (IHSt2 _ U2Has). destruct IHSt2 as [D1' [THas' Sd2]].
+      destruct (intersect_dec_label_eq _ _ Eq) as [Eq1 _].
+      lets Eql1: (subdec2_to_label_of_dec_eq Sd1).
+      lets Eql2: (subdec2_to_label_of_dec_eq Sd2).
+      rewrite <- Eq1 in Eql2. rewrite <- Eql1 in Eql2.
+      lets Eq': (typ_has_unique THas' THas Eql2). subst D1'. clear THas'.
+      exists D1. apply (conj THas).
+      apply (subdec2_intersect Sd1 Sd2 Eq).
+  + (* case subtyp_and_l *)
+    rename T2Has into T1Has, D2 into D1, H into WfT1, H0 into WfT2.
+    lets T2Has: (typ_has_total WfT2). specialize (T2Has (label_of_dec D1)).
+    destruct T2Has as [T2Hasnt | [D2 [Eq T2Has]]].
+    - exists D1. auto.
+    - destruct (intersect_dec_total _ _ Eq) as [D12 Eq12]. exists D12. split.
+      * eauto.
+      * left. apply (subdec_intersect_l _ Eq12).
+        admit. admit. (* !!! wf-less subtyp/subdec??? *)
+  + (* case subtyp_and_r *)
+    admit.
+  + (* case subtyp_or *)
+    rename T2Has into UHas.
+    specialize (IHSt1 _ UHas). destruct IHSt1 as [D01 [T1Has Sd1]].
+    specialize (IHSt2 _ UHas). destruct IHSt2 as [D02 [T2Has Sd2]].
+    lets Eql1: (subdec2_to_label_of_dec_eq Sd1).
+    lets Eql2: (subdec2_to_label_of_dec_eq Sd2).
+    rewrite <- Eql2 in Eql1.
+    destruct (union_dec_total _ _ Eql1) as [D12 Eq12]. exists D12. split.
+    - apply (typ_or_has T1Has T2Has Eq12).
+    - admit.  (*!!! *)
+  + (* case subtyp_or_l *)
+    admit.
+  + (* case subtyp_or_r *)
+    admit.
+  + (* case subtyp_trans *)
+    rename D2 into D3, T2Has into T3Has.
+    specialize (IHSt2 _ T3Has).
+    destruct IHSt2 as [D2 [T2Has Sd23]].
+    specialize (IHSt1 _ T2Has).
+    destruct IHSt1 as [D1 [T1Has Sd12]].
+    exists D1. apply (conj T1Has). apply (subdec2_trans Sd12 Sd23).
+Qed.
+
+Print Assumptions swap_sub_and_typ_has. (* !! *)
+*)
+
+(* ###################################################################### *)
+(** ** Narrowing *)
+
+Lemma narrow_binds: forall G1 x0 S1 S2 G2 x T2,
+  binds x T2 (G1 & x0 ~ S2 & G2) ->
+  subtyp (G1 & x0 ~ S1 & G2) S1 S2 ->
+  exists T1,
+    binds x T1 (G1 & x0 ~ S1 & G2) /\
+    (subtyp (G1 & x0 ~ S1 & G2) T1 T2 \/ T1 = T2).
+Proof.
+  introv Bi StS.
+  apply binds_middle_inv in Bi.
+  destruct Bi as [Bi | [[xG2 [Eq1 Eq2]]|[xG2 [Ne Bi]]]].
+  - (* case x in G2 *)
+    apply (binds_concat_right (G1 & x0 ~ S1)) in Bi.
+    exists T2. auto.
+  - (* case x = x0 *)
+    subst x0 T2. exists S1.
+    apply (conj (binds_middle_eq _ _ xG2)).
+    left. apply StS.
+  - (* case x in G1 *)
+    exists T2. refine (conj _ (or_intror eq_refl)).
+    assert (xx0: x # (x0 ~ S1)) by auto.
+    apply (binds_concat_left (binds_concat_left Bi xx0) xG2).
+Qed.
+
+Print Assumptions narrow_binds.
+
+(* Note: narrowing for typ_hasnt doesn't hold. *)
+
+Lemma narrow_typ_has:
+    forall G T D2, typ_has G T D2 -> forall G1 x S1 S2 G2,
+    G = G1 & x ~ S2 & G2 ->
+    subtyp (G1 & x ~ S1 & G2) S1 S2 ->
+    exists D1,
+      typ_has (G1 & x ~ S1 & G2) T D1 /\
+      (subdec (G1 & x ~ S1 & G2) D1 D2 \/ D1 = D2).
+Proof.
+  introv Has. induction Has; introv Eq St; subst.
+  + (* case typ_bot_has *)
+    exists (dec_bot l). split; [eauto | destruct l; simpl; eauto].
+  + (* case typ_rcd_has *)
+    exists D. eauto.
+  + (* case typ_sel_has *)
+    rename Lo into Lo2, Hi into Hi2, D into D2, T into X2.
+    specialize (IHHas1 _ _ _ _ _ eq_refl St). destruct IHHas1 as [D0 [X2Has Sd0]].
+    specialize (IHHas2 _ _ _ _ _ eq_refl St). destruct IHHas2 as [D1 [HiHas Sd]].
+    destruct Sd0 as [Sd0 | Eq].
+    - apply invert_subdec_typ_sync_left in Sd0.
+      destruct Sd0 as [Lo1 [Hi1 [Eq [StLo StHi]]]]. subst D0.
+      destruct Sd as [Sd | Eq].
+      * lets N: (narrow_binds H St). destruct N as [X1 [Bi1 StX]].
+        destruct StX as [StX | Eq].
+        { admit. (* TODO needs exp_preserves_sub *) }
+        { subst X1. rename X2 into X. exists D1. split; auto.
+          (* TODO also needs exp_preserves_sub *) admit. }
+      * subst D1. rename D2 into D. exists D.
+
+    exists D1.
+
+  + (* case typ_and_has_1 *) eauto.
+  + (* case typ_and_has_2 *) eauto.
+  + (* case typ_and_has_12 *) eauto.
+  + (* case typ_or_has *) eauto.
+
+Qed.
+
+
+
+(* ###################################################################### *)
+(** ** subtyp-and-then-lookup_tdec to lookup_tdec-and-then-subdec *)
+
+(*
 Lemma swap_sub_and_typ_has_tdec: forall G T1 T2 L Lo2 Hi2,
   subtyp G T1 T2 ->
   typ_has_tdec G T2 L Lo2 Hi2 ->
@@ -743,6 +1792,7 @@ Proof.
 Qed.
 
 Print Assumptions swap_sub_and_typ_has_tdec. (* typ_has_tdec_total!! *)
+*)
 
 
 (* ###################################################################### *)
